Internalize the inputs/outputs into the state of the freshness monad

examples/Imp2Vir/CvirSyntax.v
@@ -11,6 +11,46 @@ Import ListNotations.
 
 Section CvirSyntax.
 
+(** -- Misc -- *)
+Fixpoint mk_map (l : list block_id) (l' : list block_id) : bid_map :=
+  match l with
+  | [] => []
+  | x1::l1 => (match l' with
+             | [] => []
+             | x2::l2 => (x1,x2)::(mk_map l1 l2)
+             end)
+  end.
+
+Definition cycle {A} (l : list A) : list A :=
+    match l with
+    | [] => []
+    | x::tl => tl ++ [x]
+    end.
+
+Definition eq_bid b b' :=
+  match b,b' with
+  | Name s, Name s' => String.eqb s s'
+  | Anon n, Anon n' => @RelDec.eq_dec int eq_dec_int n n'
+  | Raw n, Raw n' => @RelDec.eq_dec int eq_dec_int n n'
+  | _,_ => false
+  end.
+
+Fixpoint find_nth' (l : list block_id) (x : block_id) (n : nat) : nat:=
+  match l with
+  | [] => 0
+  | h::t => if eq_bid x h then n else find_nth' t x (n+1)
+  end.
+
+Definition find_nth (l : list block_id) (x : block_id) := find_nth' l x 0.
+
+Lemma nth_no_error : forall {A} (l : list A) k,
+  l <> [] ->
+  nth_error l (Nat.modulo k (length l)) <> None.
+Proof.
+  intros.
+  induction l; [contradiction|].
+Admitted.
+
 Definition mk_anon (n : nat) := Anon (Z.of_nat n).
 
 Variant block_typ : Type :=
@@ -27,38 +67,34 @@ Inductive icvir : Type :=
 | Merge (_ : icvir) (_ : icvir)
 | Join (_ : nat) (_ : icvir).
 
-Definition Seq (c1 c2 : icvir) : icvir := 
+Definition Sequence (c1 c2 : icvir) : icvir :=
   Loop 1 (PermuteInputs (Merge c1 c2)).
 
-Record cvir := mk_cvir {
-    ins : list block_id;
-    outs : list block_id;
-    cfg : list (block typ);
-  }.
-
-Definition relabel_cvir (m : bid_map) (ir : cvir) : cvir :=
-  mk_cvir (ins ir) (outs ir) (ocfg_relabel m (cfg ir)).
+(* Definition If (e : texp typ) (ct cf : icvir) := *)
+(*   let cond := Block (Branch e) [] in *)
+(*   let body := Join 2 (Merge ct cf) in *)
+(*   Sequence cond body. *)
 
 From ExtLib Require Import
      Structures.Monads.
-From ITree Require Import ITree.
-From ITree Require Import Eq.
+From ITree Require Import
+     ITree
+     ITreeFacts
+     Eq.
+
+From Vellvm Require Import Tactics.
 
 Record FST := mk_FST
-  { 
+  {
+    inputs_visibles : list block_id;
+    outputs_visibles : list block_id;
     counter_reg : nat; 
     counter_bid : nat
   }.
 
-Definition fresh_init : FST := mk_FST 0 0.
+Definition fresh_init : FST := mk_FST [] [] 0 0.
 
-Definition bump_bid : FST -> FST  :=
-  fun '(mk_FST r b) => mk_FST r (S b).
-
-Definition bump_reg : FST -> FST  :=
-  fun '(mk_FST r b) => mk_FST (S r) b.
-
-Definition fresh : Type -> Type := fun X => FST -> (FST * X). 
+Definition fresh : Type -> Type := fun X => FST -> (FST * X).
 
 #[global] Instance freshM : Monad fresh := 
  {|
@@ -70,114 +106,257 @@ Import MonadNotation.
 Variable (name : nat -> block_id).
 
 Definition getReg : fresh block_id :=
-  fun '(mk_FST r b) => 
-    (mk_FST (S r) b , name r).
+  fun '(mk_FST i o r b) =>
+    (mk_FST i o (S r) b , name r).
 
 Definition getLab : fresh block_id :=
-  fun '(mk_FST r b) => 
-    (mk_FST r (S b) , name b).
+  fun '(mk_FST i o r b) =>
+    (mk_FST i o r (S b) , name b).
 
-Fixpoint mk_map (l : list block_id) (l' : list block_id) : bid_map :=
-  match l with
-  | [] => []
-  | x1::l1 => (match l' with
-             | [] => []
-             | x2::l2 => (x1,x2)::(mk_map l1 l2)
-             end)
-  end.
+Definition setInputs (inputs : list block_id) : fresh _ :=
+  fun '(mk_FST _ o r b) => (mk_FST inputs o r (S b), tt).
 
-  Definition cycle {A} (l : list A) : list A :=
-    match l with 
-    | [] => []
-    | x::tl => tl ++ [x]
-    end.
+Definition setOutputs (outputs : list block_id) : fresh _ :=
+  fun '(mk_FST i _ r b) => (mk_FST i outputs r (S b), tt).
 
-Fixpoint eval_icvir (cir : icvir) : fresh cvir :=
+Definition getInputs : fresh (list block_id) :=
+  fun '(mk_FST i o r b) =>
+    (mk_FST i o r b, i).
+
+Definition getOutputs : fresh (list block_id) :=
+  fun '(mk_FST i o r b) =>
+    (mk_FST i o r b, o).
+
+
+Fixpoint eval (cir : icvir) : fresh (list (block typ)) :=
   match cir with
 
   | Block Simple c =>
     input <- getLab;;
     output <- getLab;;
-    ret (mk_cvir [input] [output]
-                 [mk_block input [] c (TERM_Br_1 output) None]
-    )
+    setInputs [input];;
+    setOutputs [output];;
+    ret [mk_block input [] c (TERM_Br_1 output) None]
 
   | Block (Return e) c =>
     input <- getLab;;
-    ret (mk_cvir [input] [] [mk_block input [] c (TERM_Ret e) None])
+    setInputs [input];;
+    setOutputs [];;
+    ret [mk_block input [] c (TERM_Ret e) None]
 
  | Block Void c =>
     input <- getLab;;
-    ret (mk_cvir [input] [] [mk_block input [] c TERM_Ret_void None])
+    setInputs [input];;
+    setOutputs [];;
+    ret [mk_block input [] c TERM_Ret_void None]
 
  | Block (Branch e) c =>
     input <- getLab;;
     outL <- getLab;;
     outR <- getLab;;
-    ret (mk_cvir [input] [outL;outR] [mk_block input [] c (TERM_Br e outL outR) None])
+    setInputs [input];;
+    setOutputs [outL;outR];;
+    ret [mk_block input [] c (TERM_Br e outL outR) None]
 
   | PermuteInputs ir => (* Note: has been simplified. General Case? *)
-    '(mk_cvir ins outs g) <- eval_icvir ir;;
-    ret (mk_cvir
-        (cycle ins)
-        outs
-        g)
-    
-  | PermuteOutputs ir => (* Note: has been simplified. General Case? Is it useful at all anyway? *)
-    '(mk_cvir ins outs g) <- eval_icvir ir;;
-    ret (mk_cvir
-        ins
-        (cycle outs)
-        g)
-    
+    g <- eval ir;;
+    ins <- getInputs ;;
+    outs <- getOutputs ;;
+    setInputs (cycle ins);;
+    setOutputs outs;;
+    ret g
+
+  | PermuteOutputs ir => (* Note: has been simplified. General Case? *)
+    g <- eval ir;;
+    ins <- getInputs ;;
+    outs <- getOutputs ;;
+    setInputs ins;;
+    setOutputs (cycle outs);;
+    ret g
+
   | Join k ir =>
-    '(mk_cvir ins outs g) <- eval_icvir ir;;
+    g <- eval ir;;
+    ins <- getInputs ;;
+    outs <- getOutputs ;;
     merge <- getLab;;
     let rename_map := (mk_map (firstn k outs) (List.repeat merge k)) in
-    ret (mk_cvir ins                     (* inputs stays untouched *)
-                 (merge :: skipn k outs) (* we rename the k-first and don't touch the others *)
-        (ocfg_relabel rename_map g)
-    )
+    setInputs ins;;
+    setOutputs (merge :: skipn k outs);; (* we rename the k-first and don't touch the others *)
+    ret (ocfg_relabel rename_map g)
 
- | Loop k ir =>
-    '(mk_cvir ins outs g) <- eval_icvir ir;;
+  | Loop k ir =>
+    g <- eval ir;;
+    ins <- getInputs ;;
+    outs <- getOutputs ;;
     let rename_map := (mk_map (firstn k ins) (firstn k outs)) in
-    ret (mk_cvir (skipn k ins)
-                 (skipn k outs)
-                 (ocfg_relabel rename_map g))
+    setInputs (skipn k ins);;
+    setOutputs (skipn k outs);;
+    ret (ocfg_relabel rename_map g)
 
   | Merge ir1 ir2 =>
-    '(mk_cvir ins1 outs1 g1) <- eval_icvir ir1;;
-    '(mk_cvir ins2 outs2 g2) <- eval_icvir ir2;;
-    ret (mk_cvir (ins1 ++ ins2)
-                 (outs1 ++ outs2)
-                 (g1 ++ g2))
-
- end.
-
-Definition eval (cir : icvir) : fresh _ :=
-  ir <- eval_icvir cir;; 
-  ret (cfg ir). 
+    g1 <- eval ir1;;
+    ins1 <- getInputs ;;
+    outs1 <- getOutputs ;;
+    g2 <- eval ir2;;
+    ins2 <- getInputs ;;
+    outs2 <- getOutputs ;;
+    setInputs (ins1 ++ ins2);;
+    setOutputs (outs1 ++ outs2);;
+    ret (g1++g2)
+  end.
 
 Definition eval_top (cir : icvir) :=
   eval cir fresh_init.
 
 Notation conv := (convert_typ []).
 
-Definition sem (i : icvir): fresh _ :=
-   bks <- eval i;;
-   ret (denote_ocfg (conv bks)).
+From Vellvm Require Import Semantics.
+Import ITreeNotations.
 
-Lemma seq_sound : Prop. 
-refine (forall (ir1 ir2 : icvir), _ : Prop).
-refine (forall σ fto, 
-eutt eq _ _).
+Definition sem (i : icvir) : fresh _ :=
+  bks <- eval i;;
+  ret (denote_ocfg (conv bks)).
 
-refine (snd (sem (Seq ir1 ir2) σ) fto).
-refine (x <- snd (sem ir1 σ) fto;; _ (sem ir2)).
- sem (Seq ir1 ir2)) == _ (sem ir1) (sem ir2). 
+Lemma blockSimple_sound :
+  forall c σ fto,
+  eutt eq
+       (snd (sem (Block Simple c) σ) fto)
+       (let (src,target) :=
+          (snd ((input <- getLab ;;
+                 output <- getLab ;;
+                 ret (input,output)) σ)) in
+        x <- denote_code (conv c) ;; ret (inl (src,target))).
+Proof.
+  intros.
+  unfold sem.
+  simpl. repeat flatten_all.
+  simpl.
+  inv Heq.
+  inv Heq1.
+  simpl in Heq4 ; inv Heq4.
+  clear.
+Admitted.
+
+(* TODO blockRet *)
+(* TODO blockBranch *)
+(* TODO blockRetVoid *)
+
+Lemma merge_sound :
+ forall (ir1 ir2 : icvir) (σ : FST) (fto : block_id * block_id),
+ eutt eq
+      (snd (sem (Merge ir1 ir2) σ) fto)
+      (let (σ1, t1) := (sem ir1 σ) in
+       let (σ2, t2) := (sem ir2 σ1) in
+       let (_,to) := fto in
+       if (existsb (fun e => eq_bid to e) (inputs_visibles σ1))
+       then t1 fto (* the field "to" points to the left CIR *)
+       else t2 fto (* the field "to" points to the right CIR *)
+      ).
+Proof.
+  intros.
+  unfold sem.
+  simpl.
+  repeat flatten_all ; simpl ;
+  (inv Heq0;
+  inv Heq2).
+Admitted.
+
+Lemma permuteInput_sound :
+ forall (ir : icvir) (σ : FST) (fto : block_id * block_id),
+ eutt eq
+      (snd (sem (PermuteInputs ir) σ) fto)
+      (let (σ', t) := sem ir σ in
+       let inputs := inputs_visibles σ' in
+       let outputs := outputs_visibles σ' in
+       let (from, src) := fto in
+       let i := find_nth inputs src in
+       let nsrc := nth_error inputs ((i+1) mod (length inputs)) in
+       match nsrc with
+       | None => t (from, src) (* impossible because of mod *)
+       | Some nsrc => t (from, nsrc)
+end).
+Proof.
+  intros.
+  unfold sem.
+  simpl.
+  repeat flatten_goal.
+  Focus 2.
+  apply nth_no_error in Heq2. contradiction. admit.
+  cbn.
+Admitted.
 
 
+Lemma loop_sound :
+  forall (ir : icvir) (k : nat) (σ : FST) (fto : block_id * block_id),
+  eutt eq
+       (snd (sem (Loop k ir) σ) fto)
+       (let (σ', t) := sem ir σ in
+        let inputs := inputs_visibles σ' in
+        let outputs := outputs_visibles σ' in
+        (iter (C := Kleisli _)
+               (fun '(from,src) =>
+                  let (σ', t) := sem ir σ in
+                  let inputs := inputs_visibles σ' in
+                  let outputs := outputs_visibles σ' in
+                  fto' <- t (from,src) ;; (* : fto' : (bid*bid + dvalue)*)
+                  match fto' with
+                  | inr dv => ret (inr (inr dv)) (* if dvalue, stops the iter and return the value*)
+                  | inl (src,target) =>
+                    (let i := find_nth outputs target in
+                     if (Nat.ltb i k)
+                     then (
+                        match nth_error inputs (i mod (length inputs)) with
+                        | None => ret (inl (src,target)) (* TODO : raise an error *)
+                        | Some ntarget => ret (inl (src,ntarget))
+                        end)
+                     else
+                       ret (inr (inl (src,target))))
+                  end)
+               fto)).
+Proof.
+  intros.
+  unfold sem.
+  simpl.
+  repeat flatten_goal.
+Admitted.
+
+Lemma join_sound : Prop.
+  refine (
+  forall (ir : icvir) (k : nat) (σ : FST) (fto : block_id * block_id),
+  eutt eq
+       (snd (sem (Join k ir) σ) fto) _).
+  refine
+       (let (σ', t) := sem ir σ in
+        let inputs := inputs_visibles σ' in
+        let outputs := outputs_visibles σ' in
+        fto' <- t fto ;; (* : fto' : (bid*bid + dvalue)*)
+        match fto' with
+        | inr dv => ret (inr dv) (* if dvalue, stops the iter and return the value*)
+        | inl (src,target) =>
+          let i := find_nth outputs target in
+          if (Nat.ltb i k)
+          then ret (inl (src,_)) (* target new label *)
+          else ret (inl (src,target)) (* no change *)
+        end).
+Admitted.
+
+Lemma seq_sound : forall (ir1 ir2 : icvir) σ fto,
+    (snd (sem (Sequence ir1 ir2) σ) fto)
+      ≈
+      (let (σ',t) := sem ir1 σ in
+       fto' <- (t fto) ;;
+       match fto' with
+       | inr dv => ret (inr dv)
+       | inl fto' => snd (sem ir2 σ') fto'
+       end).
+Proof.
+  intros.
+  simpl.
+  unfold Sequence.
+  rewrite loop_sound.
+  simpl.
+  repeat flatten_goal.
+Admitted.
 
 
 From ExtLib Require Import
@@ -185,7 +364,6 @@ From ExtLib Require Import
      Data.Monads.OptionMonad.
 
 Import MonadNotation.
-
 
 
 From Vellvm Require Import
@@ -196,7 +374,7 @@ Import VIR_Notations.
 From Coq Require Import Strings.String.
 Require Import CompileExpr.
 
-Fixpoint compile (next_reg : int) (s : stmt) (env: StringMap.t int)
+Fixpoint compile_imp (next_reg : int) (s : stmt) (env: StringMap.t int)
   : option (int * (StringMap.t int) * icvir) :=
   match s with
   | Skip => Some(next_reg, env, Block Simple [])
@@ -205,38 +383,28 @@ Fixpoint compile (next_reg : int) (s : stmt) (env: StringMap.t int)
     ret (next_reg, env, Block Simple ir)
 
   | Seq l r =>
-    '(next_reg, env, ir_l) <- compile next_reg l env;;
-    '(next_reg, env, ir_r) <- compile next_reg r env;;
-    ret (next_reg, env, (Merge ir_l ir_r))
+    '(next_reg, env, ir_l) <- compile_imp next_reg l env;;
+    '(next_reg, env, ir_r) <- compile_imp next_reg r env;;
+    ret (next_reg, env, (Sequence ir_l ir_r))
 
   | While e b =>
     '(cond_reg, expr_ir) <- compile_cond next_reg e env;;
-    '(next_reg, _, ir) <- compile (cond_reg + 1) b env;;
-    ret (next_reg, env, ir)
+    '(next_reg, _, ir) <- compile_imp (cond_reg + 1) b env;;
+    ret (next_reg, env, ir) (* TODO *)
 
   | If e l r =>
     '(cond_reg, expr_code) <- compile_cond next_reg e env;;
-    '(next_reg, _, ir_l) <- compile (cond_reg + 1) l env;;
-    '(next_reg, _, ir_r) <- compile next_reg r env;;
-    ret (next_reg, env, ir_l)
+    '(next_reg, _, ir_l) <- compile_imp (cond_reg + 1) l env;;
+    '(next_reg, _, ir_r) <- compile_imp next_reg r env;;
+    ret (next_reg, env, ir_l) (* TODO *)
   end.
 
-Definition compile_eval (s : stmt) :=
-  '(_, _, ir) <- compile 0 s (StringMap.empty int);;
-    ret (eval_icvir 0 ir).
+Definition compile_icvir (s : stmt) :=
+  '(_, _, ir) <- compile_imp 0 s (StringMap.empty int);;
+  ret (snd (eval_top ir)).
 
-Compute (compile 0 (trivial_seq "a" "b" 42) (StringMap.empty int)).
-Compute (compile_eval (trivial_seq "a" "b" 42)).
-
-
-
+Compute (compile_imp 0 (trivial_seq "a" "b" 42) (StringMap.empty int)).
+Compute (compile_icvir (trivial_seq "a" "b" 42)).
 
 
 End CvirSyntax.
-
-(* Inductive ext_cvir (id_typ : Type) : Type := *)
-(* | Core (_ : cvir id_typ) *)
-(* | Seq (_ : ext_cvir) (_ : ext_cvir) *)
-(* | IfThenElse (branch : ext_cvir) (if_true : ext_cvir) (if_false : ext_cvir) *)
-(* | While (cond : ext_cvir). *)
-(* (* extended cvir *) *)
